src-coq/corex10_noclocks.v
@@ -12,10 +12,7 @@ Inductive asn : Type  :=
   | seq(n:nat) : asn
   | v(v:var) :asn
   | a :asn
-  | f :asn
-  | cf : asn
-  | ca : asn.
-
+  | f :asn.
 
 Inductive expr : Type :=
   | val(i:nat):expr
@@ -29,34 +26,39 @@ Inductive heap : Type :=
 (* We choose to define stmt as a function from types
   so that we can annotate a statement with any kind of value.
   In reality, we are only interested in stmt unit and stmt (List asn). *)
-Inductive stmt (A : Type) : Type:=
-| Advance(a:A) : stmt A
-| Skip(a:A) : stmt A
-| Local (e:var)(a:A) : stmt A
-| Assign (l:var) (i:expr) (r:expr)(a:A) : stmt A    (* L[I] = R *)
-| Xseq (c1:stmt A) (c2:stmt A)(a:A)  : stmt A
-| Xfor (x:var) (l:expr) (u:expr) (s:stmt A) (a:A) : stmt A
-| Async (c:stmt A)(a:A) : stmt A
-| Finish (c:stmt A)(a:A) : stmt A
-| ClockedAsync (c:stmt A)(a:A): stmt A
-| ClockedFinish (c:stmt A)(a:A) : stmt A.
+
+
+Inductive stmt (A:Type):Type:=
+  | Skip(a:A): stmt A
+  | Local (e:var)(a:A): stmt A
+  | Assign (l:var) (i:expr) (r:expr)(a:A): stmt A    (* L[I] = R *)
+  | Xseq (c1:stmt A) (c2:stmt A)(a:A): stmt A
+  | Xfor (x:var) (l:expr) (u:expr) (s:stmt A) (a:A): stmt A
+  | Async (c:stmt A)(a:A): stmt A
+  | Finish (c:stmt A)(a:A): stmt A.
+
+Definition isBasic (A:Type)(s:stmt A):Prop := 
+  match s with
+    | Skip _ => True
+    | Local _ _  => True
+    | Assign _ _ _ _  => True
+    |  _ => False
+  end.
 
 Definition ustmt := stmt unit.
 Definition pth := list asn.
-Definition annStmt := stmt pth.
+Definition ann_stmt := stmt pth.
 
-Definition advance:ustmt := Advance unit tt.
 Definition skip:ustmt := Skip unit tt.
 Definition local (e:var):ustmt := Local unit e tt.
 Definition assign (l:var)(i:expr) (r:expr):ustmt := Assign unit l i r tt.
 Definition xseq (c1:ustmt)(c2:ustmt):ustmt := Xseq unit c1 c2 tt.
 Definition xfor (x:var)(l:expr) (u:expr) (s:ustmt):ustmt := Xfor unit x l u s tt.
 Definition async (c:ustmt):ustmt := Async unit c tt.
-Definition clockedAsync (c:ustmt):ustmt := ClockedAsync unit c tt.
-Definition clockedFinish (c:ustmt):ustmt := ClockedFinish unit c tt.
+Definition finish (c:ustmt):ustmt := Finish unit c tt.
 
-Inductive path A: stmt A -> list asn -> stmt A -> Prop :=
- | path_ad : forall a, path A (Advance A a) nil (Advance A a)
+
+Inductive path A: stmt A -> pth -> stmt A -> Prop :=
  | path_skip: forall a, path A (Skip A a) nil (Skip A a)
  | path_local: forall a V, path A (Local A V a) nil (Local A V a)
  | path_assign: forall a L I R, path A  (Assign A L I R a) nil (Assign A L I R a)
@@ -64,13 +66,27 @@ Inductive path A: stmt A -> list asn -> stmt A -> Prop :=
  | path_seq1:  forall a S T P U, path A S P U -> path A (Xseq A T S a) ((seq 1)::  P) U
  | path_x: forall a X L H U S P, path A S P U -> path A (Xfor A X L H S a) ((v X) :: P) U
  | path_a: forall aa S P U, path A S P U -> path A (Async A S aa) (a :: P) U
- | path_f: forall a S P U, path A S P U -> path A (Finish A S a)  (f ::P) U
- | path_ca: forall a S P U, path A S P U -> path A (ClockedAsync A S a) (ca:: P) U
- | path_cf: forall a S P U, path A S P U -> path A (ClockedFinish A S a) (cf :: P) U.
+ | path_f: forall a S P U, path A S P U -> path A (Finish A S a)  (f ::P) U.
 
-Fixpoint ann2 (s:ustmt) (p: list asn):annStmt  :=
+Definition hasBasicPath (s: ustmt)(p:pth): Prop := exists q, (path unit s p q) /\ isBasic unit q.
+
+Inductive cft: pth -> Prop :=
+  | cft_nil: cft nil
+  | cft_f: forall p, cft (f::p)
+  | cft_rec: forall n p, cft p -> cft (seq(n)::p).
+
+Inductive hb01: pth -> pth -> Prop :=
+  | hb01_seq: forall p q, cft q -> hb01 (seq(0)::p) (seq(1)::q)
+  | hb01_rec: forall a p q, hb01 p q -> hb01 (a::p) (a::q).
+
+Definition hb0(s:ustmt)(p:pth)(q:pth): Prop := hasBasicPath s p /\ hasBasicPath s q /\ hb01 p q.
+
+Inductive precedes A: A -> A -> list A -> Prop :=
+  | precedes_rec: forall a b c r, precedes A a b r -> precedes A a b (c::r)
+  | precedes_base: forall a b rf rt,  precedes A a b (a::rf ++ b::rt).
+
+Fixpoint ann2 (s:ustmt) (p:pth):ann_stmt  :=
   match s with
-   | Advance x => Advance pth p
    | Skip x =>  Skip pth p
    | Local e x =>  Local pth e p
    | Assign l i r x => Assign pth  l i r p
@@ -78,11 +94,9 @@ Fixpoint ann2 (s:ustmt) (p: list asn):annStmt  :=
    | Async s x => Async pth (ann2 s (p ++ a::nil)) p
    | Finish s x =>  Finish pth (ann2 s (p ++  f::nil)) p
    | Xseq s0 s1 x=> Xseq pth  (ann2 s0 ( p ++ (seq 0)::nil)) (ann2  s1(p ++ (seq 1)::nil)) p
-   | ClockedAsync s x => ClockedAsync pth (ann2 s (p ++ ca::nil)) p
-   | ClockedFinish s x => ClockedFinish pth (ann2 s (p ++ cf::nil)) p
 end.
 
-Definition annotate (s:ustmt) : annStmt :=  ann2 s nil.
+Definition annotate (s:ustmt) : ann_stmt :=  ann2 s nil.
 
 Definition eq_nat : forall (x y:nat), {x=y}+{x<>y}.
 Proof. decide equality. Qed.
@@ -95,7 +109,6 @@ Fixpoint substE (e:expr)(v:var)(e0:expr):expr :=
 
 Fixpoint substS (A:Type)(s:stmt A)(v:var)(e:expr):(stmt A)  :=
   match s  with
-   | Advance x => Advance A x
    | Skip x =>  Skip A x
    | Local e x =>  Local A e x
    | Assign l i r x => Assign A l (substE i v e) (substE r v e) x
@@ -103,60 +116,24 @@ Fixpoint substS (A:Type)(s:stmt A)(v:var)(e:expr):(stmt A)  :=
    | Async s x => Async A (substS A s v e) x
    | Finish s x =>  Finish A (substS A s v e) x
    | Xseq s0 s1 x=> Xseq A (substS A s0 v e) (substS A s1 v e) x
-   | ClockedAsync s x => ClockedAsync A (substS A s v e) x
-   | ClockedFinish s x => ClockedFinish A (substS A s v e) x
 end.
 Axiom x:var.
 
 Inductive isAsync A: stmt A  -> Prop := 
   | isAsync_a:forall S x,  isAsync A (Async A S x)
-  | isAsync_ca: forall S x, isAsync A (ClockedAsync A S x)
   | isAsync_s: forall S0 S1 a, isAsync A S0 -> isAsync A S1  -> isAsync A (Xseq A S0 S1 a)
-  | isAsync_X: forall S0 z l u a, isAsync A S0  -> isAsync A (Xfor _ z l u S0 a) 
-.
+  | isAsync_X: forall S0 z l u a, isAsync A S0  -> isAsync A (Xfor _ z l u S0 a).
 
 Inductive isSync A: stmt A  -> Prop := 
-  | isSync_ad: forall a, isSync A (Advance A a)
   | isSync_sk: forall a, isSync A (Skip A a)
   | isSync_local: forall e a, isSync A (Local A e a)
   | isSync_ass: forall l i r a, isSync A (Assign A l i r a)
   | isSync_a:forall S x,  isSync A (Finish A S x)
-  | isSync_ca: forall S x, isSync A (ClockedFinish A S x)
   | isSync_s0: forall S0 S1 a, isSync A S0  -> isSync A (Xseq A S0 S1 a)
   | isSync_s1: forall S0 S1 a, isSync A S1  -> isSync A (Xseq A S0 S1 a)
-  | isSync_X: forall S0 z l u a, isSync A S0  -> isSync A (Xfor _ z l u S0 a) 
-.
+  | isSync_X: forall S0 z l u a, isSync A S0  -> isSync A (Xfor _ z l u S0 a).
 
-Theorem sync_or_async: forall A S, (isSync A S) \/ (isAsync A S).
-Proof.  
-induction S. (* a simple reasonning by case is not enough, we need induction *)
-  - left; constructor.
-  - left; constructor.
-  - left; constructor.
-  - left; constructor.
-  - destruct IHS1.
-    + left; constructor; auto.
-    + destruct IHS2.
-      * left; apply isSync_s1; auto. (* [constructor] will chose the first possible case, but this a dead-end *)
-      * right; constructor; auto.
-  - destruct IHS.
-    + left; constructor; auto.
-    + right; constructor; auto.
-  - destruct IHS.
-    + right; constructor; auto.
-    + right; constructor; auto.
-  - destruct IHS.
-    + left; constructor; auto.
-    + left; constructor; auto.
-  - destruct IHS.
-    + right; constructor; auto.
-    + right; constructor; auto.
-  - destruct IHS.
-    + left; constructor; auto.
-    + left; constructor; auto.
-Qed.
-
-Theorem sync_or_async2: forall A S, (isSync A S) \/ (isAsync A S). (* The same proof with more automation *)
+Theorem sync_or_async: forall A S, (isSync A S) \/ (isAsync A S).  (* The same proof with more automation *)
 
 (* A custom tactic I use very often (a bit simplified here) *)
 Ltac go := 
@@ -175,19 +152,8 @@ Proof.
   induction S; intuition; go. 
 Qed.
 
-Inductive hasYield: annStmt -> annStmt -> bool -> Prop :=
-  | hasYield_ad: forall p, hasYield (Advance pth p)(Skip pth p) true
-  | hasYield_ca: forall S SS p B, hasYield S SS B 
-    -> hasYield (ClockedAsync pth S p) (ClockedAsync pth SS p) B
-  | hasYield_seq_syn: forall S T SS B p,
-    hasYield S SS B -> isSync pth S -> hasYield (Xseq pth S T p)(Xseq pth SS T p) B
-  | hasYield_seq_asyn: forall S T TT SS  B1 B2 p, 
-                         hasYield S SS B1 -> hasYield T TT B2 -> isAsync pth S 
-                         -> hasYield (Xseq pth S T p)(Xseq pth SS T p) (orb B1 B2)
-  | hasYield_async: forall S SS p, hasYield (Async pth S p) (Async pth SS p) false.
-
 Inductive config: Type :=
-  | c(a:annStmt)(h:heap):config
+  | c(a:ann_stmt)(h:heap):config
   | t(h:heap): config.
 
 
@@ -203,22 +169,12 @@ Inductive deriv: config -> config -> pth -> Prop :=
     deriv (c s h) (t hh) p -> deriv (c (Async pth s p) h) (t hh) p
   | deriv_f: forall s h hh p, 
     deriv (c s h) (t hh) p -> deriv (c (Finish pth s p) h) (t hh) p
-  | deriv_ca: forall s h hh p, 
-    deriv (c s h) (t hh) p -> deriv (c (ClockedAsync pth s p) h) (t hh) p
-  | deriv_cf: forall s h hh p, 
-    deriv (c s h) (t hh) p -> deriv (c (ClockedFinish pth s p) h) (t hh) p
   | deriv_for: forall s x h lo hi p, 
     lo > hi  -> deriv (c (Xfor pth x (val lo) (val hi) s p) h) (t h) p
   | deriv_a_r: forall s ss h hh p q, 
     deriv (c s h) (c ss hh) p -> deriv (c (Async pth s q) h) (c (Async pth ss q) hh) p
-  | deriv_ca_r: forall s ss h hh p q, 
-    deriv (c s h) (c ss hh) p -> deriv (c (ClockedAsync pth s q) h) (c (ClockedAsync pth ss q) hh) p
   | deriv_f_r: forall s ss h hh p q, 
     deriv (c s h) (c ss hh) p -> deriv (c (Finish pth s q) h) (c (Finish pth ss q) hh) p
-  | deriv_cf_r: forall s ss h hh p q, 
-    deriv (c s h) (c ss hh) p -> deriv (c (ClockedFinish pth s q) h) (c (ClockedFinish pth ss q) hh) p
-  | deriv_cf_a: forall s ss h hh p q, 
-    hasYield s ss true -> deriv (c (ClockedFinish pth s q) h) (c (ClockedFinish pth ss q) hh) p
   | deriv_seqr_l: forall r s h hh rr p q, 
     deriv (c r h) (c rr hh) p -> deriv (c (Xseq pth r s q) h) (c (Xseq pth rr s q) hh) p
   | deriv_aseqr: forall s ss r h hh p q, 
@@ -236,10 +192,13 @@ Inductive reduce: config -> config -> list pth -> Prop :=
 Inductive starReduce: ustmt -> heap -> list pth -> Prop := 
   | starRed: forall s h ps, reduce (c (annotate s) null) (t h) ps -> starReduce s h ps.
   
+Theorem no_stuck: forall s, exists h ps, starReduce s h ps.
 
+Lemma hb0_implies_precedence: 
+  forall s p q,  hb0 s p q -> forall h ls, starReduce s h ls -> precedes pth p q ls.
 
-Check clockedFinish skip.
-Check clockedFinish (xseq  (assign x (val 0) (val 0)) (clockedAsync skip)).
+Lemma precedence_implies_hb0: 
+  forall s p q,  (forall h ls, starReduce s h ls -> precedes pth p q ls) -> hb0 s p q.
 
-
-
+Theorem hb0_characterization: 
+  forall s p q,  hb0 s p q <-> (forall h ls, starReduce s h ls -> precedes pth p q ls).
